Fixed invariant and progressed on proof - Simplified the munch step to figure out the correct invariant first

compiler/backend/proofs/word_instProofScript.sml
@@ -15,7 +15,7 @@ val flatten_exp_ok = prove(``
   fs[flatten_exp_def]
   >-
     (fs[flatten_exp_def,word_exp_def]>>LET_ELIM_TAC>>
-    `ws = ws'` by 
+    `ws = ws'` by
       (match_mp_tac LIST_EQ>>unabbrev_all_tac>>fs[EL_MAP,EL_MEM])>>
     metis_tac[])
   >>
@@ -25,10 +25,10 @@ val flatten_exp_ok = prove(``
 
 (*All ops are 2 args. Technically, we should probably check that Sub has 2 args. However, the semantics already checks that and it will get removed later*)
 val binary_branch_exp_def = tDefine "binary_branch_exp" `
-  (binary_branch_exp (Op Sub exps) = EVERY (binary_branch_exp) exps) ∧ 
+  (binary_branch_exp (Op Sub exps) = EVERY (binary_branch_exp) exps) ∧
   (binary_branch_exp (Op op xs) = (LENGTH xs = 2 ∧ EVERY (binary_branch_exp) xs)) ∧
-  (binary_branch_exp (Load exp) = binary_branch_exp exp) ∧ 
-  (binary_branch_exp (Shift shift exp nexp) = binary_branch_exp exp) ∧  
+  (binary_branch_exp (Load exp) = binary_branch_exp exp) ∧
+  (binary_branch_exp (Shift shift exp nexp) = binary_branch_exp exp) ∧
   (binary_branch_exp exp = T)`
   (WF_REL_TAC `measure (exp_size ARB)`
    \\ REPEAT STRIP_TAC \\ IMP_RES_TAC MEM_IMP_exp_size
@@ -42,101 +42,190 @@ val flatten_exp_binary_branch_exp = prove(``
   binary_branch_exp (flatten_exp exp)``,
   ho_match_mp_tac flatten_exp_ind>>fs[flatten_exp_def,binary_branch_exp_def,EVERY_MEM,EVERY_MAP])
 
+val flatten_exp_every_var_exp = prove(``
+  ∀exp.
+  every_var_exp P exp ⇒
+  every_var_exp P (flatten_exp exp)``,
+  ho_match_mp_tac flatten_exp_ind>>fs[flatten_exp_def,every_var_exp_def,EVERY_MEM,EVERY_MAP])
+
 val num_exp_equiv = prove(``
   word_inst$num_exp = wordSem$num_exp``,
   fs[FUN_EQ_THM]>>Induct>>
   fs[wordSemTheory.num_exp_def,word_instTheory.num_exp_def])
 
-(*2nd step: Convert expressions to insts*)
-val inst_select_exp_thm = prove(``
-  ∀tar temp exp s w.
-  binary_branch_exp exp ∧ 
-  word_exp s exp = SOME w ⇒ 
-  let (res,s') = evaluate ((inst_select_exp tar temp exp),s) in
-    res = NONE ∧
-    s' = s with locals:= s'.locals ∧ 
-    ∀x. 
-    if x = tar then lookup x s'.locals = SOME (Word w)
-    else if x < temp then lookup x s'.locals = lookup x s.locals
-    else T``,
-  ho_match_mp_tac inst_select_exp_ind>>
-  rpt strip_tac>>
-  fs[LET_THM,inst_select_exp_def,evaluate_def,word_exp_def,inst_def,assign_def,set_var_def,lookup_insert,get_vars_def,set_vars_def,get_var_def,binary_branch_exp_def,binary_branch_exp_def]
-  >-(EVERY_CASE_TAC>>fs[alist_insert_def,lookup_insert])
-  >-(EVERY_CASE_TAC>>fs[alist_insert_def,lookup_insert])
+val locals_rel_def = Define`
+  locals_rel temp (s:'a word_loc num_map) t ⇔ (∀x. x < temp ⇒ lookup x s = lookup x t)`
+
+val locals_rel_word_exp = prove(``
+  ∀s exp w.
+  every_var_exp (λx. x < temp) exp ∧
+  word_exp s exp = SOME w ∧
+  locals_rel temp s.locals loc ⇒
+  word_exp (s with locals:=loc) exp = SOME w``,
+  ho_match_mp_tac word_exp_ind>>rw[]>>
+  fs[word_exp_def,every_var_exp_def,locals_rel_def]
   >-
-    (EVERY_CASE_TAC>>fs[binary_branch_exp_def]>>
-    res_tac>>
-    qpat_abbrev_tac`A = evaluate (B,C)`>>
-    Cases_on`A`>>fs[]>>
-    `lookup temp r.locals = SOME (Word x)` by metis_tac[]>>
-    fs[word_op_def,mem_load_def,state_component_equality,lookup_insert]>>
-    rw[]>>Cases_on`x'=tar`>>fs[]>>
-    rw[]>>first_x_assum(qspec_then `x'` assume_tac)>>
-    `x' ≠ temp` by 
-      (res_tac>>DECIDE_TAC)>>
-    `x' < temp+1` by DECIDE_TAC>>
-    metis_tac[])
+    (EVERY_CASE_TAC>>
+    res_tac>>fs[])
   >-
-    cheat
-    (*Cases_on`op`>>fs[binary_branch_exp_def,IS_SOME_EXISTS]>>
-    EVERY_CASE_TAC>>res_tac>>
-    qpat_abbrev_tac`A=evaluate(B,C)`>>
-    Cases_on`A`>>fs[]>>
-    (*TODO: Strengthen IH so that this is true*)
-    `word_exp r exp' = SOME x'` by cheat>>
-    res_tac>>
-    qpat_abbrev_tac`A=evaluate(B,C)`>>
-    Cases_on`A`>>fs[]>>
-    cheat*)
+    (qpat_assum`A= SOME w` mp_tac>>FULL_CASE_TAC>>fs[mem_load_def])
   >-
-    (EVERY_CASE_TAC>>fs[binary_branch_exp_def]>>
-    res_tac>>
-    qpat_abbrev_tac`A = evaluate (B,C)`>>
-    Cases_on`A`>>fs[]>>
-    `lookup temp r.locals = SOME (Word x)` by metis_tac[]>>
-    fs[word_op_def,mem_load_def,state_component_equality,lookup_insert,Once num_exp_def,num_exp_equiv]>>
-    rw[]>>Cases_on`x'=tar`>>fs[]>>
-    rw[]>>first_x_assum(qspec_then `x'` assume_tac)>>
-    `x' ≠ temp` by 
-      (res_tac>>DECIDE_TAC)>>
-    `x' < temp+1` by DECIDE_TAC>>
+    (qpat_assum`A= SOME w` mp_tac>>
+    LET_ELIM_TAC>>
+    Cases_on`EVERY IS_SOME ws`>>fs[]>>
+    `ws = ws'` by
+      (unabbrev_all_tac>>
+      fs[LIST_EQ,MAP_EQ_f,EVERY_MEM,MEM_MAP,IS_SOME_EXISTS]>>rw[]>>
+      res_tac>>fs[])>>
     metis_tac[])
   >>
-    Cases_on`v11`>>fs[binary_branch_exp_def,word_op_def])
-
-val locals_rel_def = Define`
-  locals_rel s t ⇔ (∀x v. lookup x s = SOME v ⇒ lookup x t = SOME v)` 
+    EVERY_CASE_TAC>>res_tac>>fs[])
+     
+(*2nd step: Convert expressions to insts*)
+val inst_select_exp_thm = prove(``
+  ∀c tar temp exp s w loc.
+  binary_branch_exp exp ∧
+  every_var_exp (λx. x < temp) exp ∧
+  locals_rel temp s.locals loc ∧
+  word_exp s exp = SOME w
+  ⇒
+  ∃loc'.
+  evaluate ((inst_select_exp c tar temp exp),s with locals:=loc) = (NONE:'a result option,s with locals:=loc') ∧
+  ∀x.
+    if x = tar then lookup x loc' = SOME (Word w)
+    else if x < temp then lookup x loc' = lookup x s.locals
+    else T``,
+  ho_match_mp_tac inst_select_exp_ind>>
+  fs[inst_select_exp_def,evaluate_def,binary_branch_exp_def,every_var_exp_def]>>
+  rpt strip_tac
+  >-
+    (*TODO: Will be replaced by munched version*)
+    (fs[GSYM AND_IMP_INTRO,word_exp_def]>>EVERY_CASE_TAC>>fs[]>>
+    first_assum(fn th => first_x_assum(mp_tac o C MATCH_MP th)) >>
+    simp[LET_THM,evaluate_def]>>rw[]>>
+    `lookup temp loc' = SOME (Word x)` by metis_tac[]>>
+    simp[inst_def,assign_def,word_exp_def,word_op_def]>>fs[mem_load_def]>>
+    simp[state_component_equality,set_var_def,lookup_insert]>>
+    rw[]>>DISJ2_TAC>>strip_tac>>
+    `x' ≠ temp` by DECIDE_TAC>>metis_tac[])
+  >-
+    (fs[LET_THM,evaluate_def,inst_def,assign_def,word_exp_def,set_var_def,mem_load_def,word_op_def]>>
+    simp[state_component_equality,locals_rel_def,lookup_insert]>>
+    fs[locals_rel_def])
+  >-
+    (fs[LET_THM,evaluate_def,inst_def,assign_def,word_exp_def,set_var_def,mem_load_def,word_op_def,get_vars_def,set_vars_def,get_var_def]>>
+    fs[locals_rel_def]>>pop_assum mp_tac>>ntac 2 FULL_CASE_TAC>>fs[]>>
+    res_tac>>fs[alist_insert_def]>>rw[]>>
+    simp[state_component_equality,lookup_insert])
+  >-
+    (fs[LET_THM,evaluate_def,inst_def,assign_def,word_exp_def,set_var_def,mem_load_def,word_op_def,get_vars_def,set_vars_def,get_var_def]>>
+    FULL_CASE_TAC>>fs[]>>pop_assum mp_tac>>FULL_CASE_TAC>>fs[locals_rel_def]>>
+    simp[state_component_equality,lookup_insert])
+  >-
+    (*TODO: Will be replaced by munched version
+      But this shows that the invs work for multiple temporaries
+    *)
+    (`binary_branch_exp exp ∧ binary_branch_exp exp'` by 
+      (Cases_on`op`>>fs[binary_branch_exp_def])>>
+    fs[word_exp_def,LET_THM,IS_SOME_EXISTS]>>
+    first_x_assum(qspecl_then[`s`,`x`,`loc`] assume_tac)>>rfs[evaluate_def]>>
+    simp[LET_THM,inst_def,assign_def]>>
+    first_x_assum(qspecl_then[`s with locals:= loc'`,`x'`,`loc'`] mp_tac)>>
+    fs[]>>discharge_hyps>-
+      (rw[locals_rel_def]
+      >-
+        (match_mp_tac every_var_exp_mono>>
+        HINT_EXISTS_TAC>>fs[]>>DECIDE_TAC)
+      >>
+        (*word_exp invariant under extra locals*)
+        match_mp_tac locals_rel_word_exp>>
+        fs[locals_rel_def]>>
+        rw[]>>`x'' ≠ temp` by DECIDE_TAC>>
+        metis_tac[])
+    >>
+      strip_tac>>fs[word_exp_def]>>
+      `lookup temp loc'' = SOME (Word x) ∧
+       lookup (temp+1) loc'' = SOME (Word x')` by
+         (first_assum(qspecl_then[`temp`] assume_tac)>>
+         first_x_assum(qspecl_then[`temp+1`] assume_tac)>>
+         `temp ≠ temp+1` by DECIDE_TAC>>
+         fs[]>>metis_tac[])>>
+      simp[LET_THM,state_component_equality,set_var_def,lookup_insert]>>
+      rw[]>>DISJ2_TAC>>strip_tac>>
+      `x''<temp+1 ∧ x'' ≠ temp ∧ x'' ≠ temp+1` by DECIDE_TAC>>
+      metis_tac[])
+  >-
+    (fs[GSYM AND_IMP_INTRO,word_exp_def]>>EVERY_CASE_TAC>>fs[]>>
+    first_assum(fn th => first_x_assum(mp_tac o C MATCH_MP th)) >>
+    simp[]>>strip_tac>>
+    simp[evaluate_def,inst_def,word_exp_def,assign_def,num_exp_def]>>
+    `lookup temp loc' = SOME (Word x)` by metis_tac[]>>
+    fs[num_exp_equiv,set_var_def,state_component_equality,lookup_insert]>>
+    rw[]>>DISJ2_TAC>>strip_tac>>
+    `x' ≠ temp` by DECIDE_TAC>>
+    metis_tac[])
+  >>
+    fs[LET_THM,evaluate_def,inst_def,assign_def,word_exp_def,set_var_def,mem_load_def,word_op_def,get_vars_def,set_vars_def,get_var_def]>>
+    Cases_on`v14`>>fs[binary_branch_exp_def])
 
 val locals_rel_get_vars  = prove(``
   ∀ls vs.
-  get_vars ls st = SOME vs ∧ 
-  locals_rel st.locals loc ⇒ 
+  get_vars ls st = SOME vs ∧
+  EVERY (λx. x < temp) ls ∧
+  locals_rel temp st.locals loc ⇒
   get_vars ls (st with locals:= loc) = SOME vs``,
   Induct>>fs[get_vars_def]>>rw[]>>
-  EVERY_CASE_TAC>>fs[locals_rel_def,get_var_def]>>
-  metis_tac[option_CLAUSES])
+  qpat_assum`A=SOME vs` mp_tac>>ntac 2 FULL_CASE_TAC>>rw[]>>
+  res_tac>>fs[get_var_def,locals_rel_def]>>
+  res_tac>>
+  fs[])
 
 val locals_rel_alist_insert = prove(``
   ∀ls vs s t.
-  locals_rel s t ⇒ 
-  locals_rel (alist_insert ls vs s) (alist_insert ls vs t)``,
+  locals_rel temp s t ∧
+  EVERY (λx. x < temp) ls ⇒
+  locals_rel temp (alist_insert ls vs s) (alist_insert ls vs t)``,
   ho_match_mp_tac alist_insert_ind>>fs[alist_insert_def,locals_rel_def]>>
   rw[]>>
   Cases_on`x'=ls`>>fs[lookup_insert])
 
-(*Simple thm for cases where we do not change the program
-Note: This can be directly proved by instantiating evaluate_apply_colour
-but the form of the theorem isn't nice (because of permutations)
+val locals_rel_get_var = prove(``
+  r < temp ∧
+  get_var r st = SOME x ∧
+  locals_rel temp st.locals loc ⇒
+  get_var r (st with locals:=loc) = SOME x``,
+  fs[get_var_def,locals_rel_def]>>
+  metis_tac[])
+
+val locals_rel_get_var_imm = prove(``
+  every_var_imm (λx.x<temp) r ∧
+  get_var_imm r st = SOME x ∧
+  locals_rel temp st.locals loc ⇒
+  get_var_imm r (st with locals:=loc) = SOME x``,
+  Cases_on`r`>>fs[get_var_imm_def,every_var_imm_def]>>
+  metis_tac[locals_rel_get_var])
+
+val locals_rel_set_var = prove(``
+  ∀n s t.
+  locals_rel temp s t ⇒ 
+  locals_rel temp (insert n v s) (insert n v t)``,
+  rw[]>>fs[locals_rel_def,lookup_insert])
+
+(*Extra temporaries not mentioned in program
+  do not affect evaluation
+  This is extra work, but might be helpful in props?
+  Otherwise, just prove it together with the inst
+  select thm
 *)
-val locals_rel_eval_thm = prove(``
-  ∀prog st res rst loc.
+val locals_rel_evaluate_thm = prove(``
+  ∀prog st res rst loc temp.
   evaluate (prog,st) = (res,rst) ∧
   res ≠ SOME Error ∧
-  locals_rel st.locals loc ⇒
+  every_var (λx.x < temp) prog ∧
+  locals_rel temp st.locals loc ⇒
   ∃loc'.
   evaluate (prog,st with locals:=loc) = (res,rst with locals:=loc') ∧
-  locals_rel rst.locals loc'``,
+  locals_rel temp rst.locals loc'``,
   completeInduct_on`prog_size (K 0) prog`>>
   rpt strip_tac>>
   Cases_on`prog`>>
@@ -144,48 +233,68 @@ val locals_rel_eval_thm = prove(``
   >-
     metis_tac[]
   >-
-    (qpat_assum `A = (res,rst)` mp_tac>> ntac 2 FULL_CASE_TAC>>fs[]>>
+    (qpat_assum `A = (res,rst)` mp_tac>> ntac 2 FULL_CASE_TAC>>
+    fs[every_var_def]>>
     imp_res_tac locals_rel_get_vars>>
     fs[set_vars_def]>>imp_res_tac locals_rel_alist_insert>>
     fs[state_component_equality]>>
     rw[]>>metis_tac[])
+  >-
+    (Cases_on`i`>>fs[inst_def,every_var_def,every_var_inst_def]
+    >-
+      metis_tac[]
+    >-
+      (fs[assign_def,word_exp_def,set_var_def]>>
+      imp_res_tac locals_rel_set_var>>
+      fs[state_component_equality]>>
+      metis_tac[])
+    >>
+      cheat)
+  >-
+    (every_case_tac>>imp_res_tac locals_rel_word_exp>>fs[every_var_def]>>
+    rfs[state_component_equality,set_var_def]>>
+    qpat_assum`A=rst.locals` sym_sub_tac>>
+    metis_tac[locals_rel_set_var])
   >>
     cheat)
-
-val locals_rel_get_var = prove(``
-  get_var r st = SOME x ∧ 
-  locals_rel st.locals loc ⇒ 
-  get_var r (st with locals:=loc) = SOME x``,
-  fs[get_var_def,locals_rel_def])
-
-val locals_rel_get_var_imm = prove(``
-  get_var_imm r st = SOME x ∧ 
-  locals_rel st.locals loc ⇒ 
-  get_var_imm r (st with locals:=loc) = SOME x``,
-  Cases_on`r`>>fs[get_var_imm_def]>>
-  metis_tac[locals_rel_get_var])
 
 val inst_select_thm = prove(``
   ∀c temp prog st res rst loc.
   evaluate (prog,st) = (res,rst) ∧
-  every_var (λx. x < temp) prog ∧   
+  every_var (λx. x < temp) prog ∧
   res ≠ SOME Error ∧
-  locals_rel st.locals loc ⇒
-  ∃loc'. 
+  locals_rel temp st.locals loc ⇒
+  ∃loc'.
   evaluate (inst_select c temp prog,st with locals:=loc) = (res,rst with locals:=loc') ∧
-  locals_rel rst.locals loc'``,
+  locals_rel temp rst.locals loc'``,
   ho_match_mp_tac inst_select_ind>>rw[]>>
-  fs[inst_select_def,locals_rel_eval_thm]
+  fs[inst_select_def,locals_rel_evaluate_thm]
   >-
-    (*Assign*)
+    (fs[evaluate_def]>>last_x_assum mp_tac>>FULL_CASE_TAC>>rw[]>>
+    fs[every_var_def]>>imp_res_tac flatten_exp_every_var_exp>>
+    fs[Once flatten_exp_ok]>>
+    assume_tac flatten_exp_binary_branch_exp>>
+    imp_res_tac inst_select_exp_thm>>rfs[]>>
+    first_x_assum(qspecl_then[`c'`,`c`] assume_tac)>>fs[]>>
+    simp[state_component_equality,set_var_def,locals_rel_def]>>
+    rw[]>>fs[lookup_insert]>>Cases_on`x'=c'`>>fs[]>>
+    metis_tac[])
+  >-
+    (fs[evaluate_def]>>last_x_assum mp_tac>>
+    FULL_CASE_TAC>>fs[]>>strip_tac>>
+    fs[every_var_def]>>imp_res_tac flatten_exp_every_var_exp>>
+    fs[Once flatten_exp_ok]>>
+    assume_tac flatten_exp_binary_branch_exp>>
+    imp_res_tac inst_select_exp_thm>>rfs[]>>
+    first_x_assum(qspecl_then[`temp`,`c`] assume_tac)>>fs[]>>
+    fs[LET_THM,evaluate_def,word_exp_def]>>
+    first_assum(qspec_then`temp` assume_tac)>>fs[set_store_def]>>
+    fs[state_component_equality,locals_rel_def]>>
+    rw[]>>`x' ≠ temp` by DECIDE_TAC>>metis_tac[])
+  >-
+    (*undo the munched version*)
     cheat
   >-
-    (*Set*)
-    cheat
-  >-
-    (*Store*)
-    cheat
-  >- 
     (*Seq*)
     (fs[evaluate_def,LET_THM]>>Cases_on`evaluate(prog,st)`>>
     fs[every_var_def,GSYM AND_IMP_INTRO]>>
@@ -195,64 +304,70 @@ val inst_select_thm = prove(``
     IF_CASES_TAC>>fs[]>>
     metis_tac[])
   >-
-    (fs[evaluate_def]>>ntac 4 (pop_assum mp_tac)>>ntac 4 FULL_CASE_TAC>>fs[]>>
+    (fs[evaluate_def]>>ntac 4 (pop_assum mp_tac)>>ntac 4 FULL_CASE_TAC>>
+    fs[every_var_def]>>
     rw[]>> imp_res_tac locals_rel_get_var>>
     imp_res_tac locals_rel_get_var_imm>>fs[GSYM AND_IMP_INTRO,every_var_def])
-  >>
+  >-
+    (*Long proof, but should just need to unwind and apply the IH
+      on the state itself, noting that locals_rel is reflexive*)
     cheat)
 
-(*No expressions nesting*)
+(*No expressions nesting
+  TODO: Probably rename this and add the inst_ok bits to it
+  Alternatively, add another every_inst condition
+*)
 val flat_exp_conventions_def = Define`
   (*These should be converted to Insts*)
   (flat_exp_conventions (Assign v exp) = F) ∧
-  (flat_exp_conventions (Store exp num) = F) ∧ 
+  (flat_exp_conventions (Store exp num) = F) ∧
   (*The only place where top level (expression) vars are allowed*)
-  (flat_exp_conventions (Set store_name (Var r)) = T) ∧ 
+  (flat_exp_conventions (Set store_name (Var r)) = T) ∧
   (flat_exp_conventions (Set store_name _) = F) ∧
   (flat_exp_conventions (Seq p1 p2) =
     (flat_exp_conventions p1 ∧ flat_exp_conventions p2)) ∧
   (flat_exp_conventions (If cmp r1 ri e2 e3) =
-    (flat_exp_conventions e2 ∧ 
-    flat_exp_conventions e3)) ∧ 
+    (flat_exp_conventions e2 ∧
+    flat_exp_conventions e3)) ∧
   (flat_exp_conventions (Call ret dest args h) =
     ((case ret of
       NONE => T
-    | SOME (v,cutset,ret_handler,l1,l2) => 
-        flat_exp_conventions ret_handler) ∧ 
-    (case h of 
+    | SOME (v,cutset,ret_handler,l1,l2) =>
+        flat_exp_conventions ret_handler) ∧
+    (case h of
       NONE => T
-    | SOME (v,prog,l1,l2) => flat_exp_conventions prog))) ∧ 
+    | SOME (v,prog,l1,l2) => flat_exp_conventions prog))) ∧
   (flat_exp_conventions _ = T)`
 
 val inst_select_exp_conventions = prove(``
-  ∀tar temp exp.
-  flat_exp_conventions (inst_select_exp tar temp exp)``,
-  ho_match_mp_tac inst_select_exp_ind>>rw[]>>fs[inst_select_exp_def,flat_exp_conventions_def,LET_THM]>>
-  ho_match_mp_tac FOLDL_invariant>>fs[flat_exp_conventions_def])
+  ∀c tar temp exp.
+  flat_exp_conventions (inst_select_exp c tar temp exp)``,
+  ho_match_mp_tac inst_select_exp_ind>>rw[]>>fs[inst_select_exp_def,flat_exp_conventions_def,LET_THM])
 
 val inst_select_conventions = prove(``
-  ∀temp prog.
-  flat_exp_conventions (inst_select temp prog)``,
+  ∀c temp prog.
+  flat_exp_conventions (inst_select c temp prog)``,
   ho_match_mp_tac inst_select_ind >>rw[]>>
   fs[flat_exp_conventions_def,inst_select_def,LET_THM]>>
   EVERY_CASE_TAC>>
+  fs[flat_exp_conventions_def]>>
   metis_tac[inst_select_exp_conventions])
 
 (*3rd step: 3 to 2 reg if necessary*)
 
 val distinct_tar_reg_def = Define`
-  (distinct_tar_reg (Arith (Binop bop r1 r2 ri)) 
-    ⇔ (r1 ≠ r2 ∧ case ri of (Reg r3) => r1 ≠ r3 | _ => T)) ∧ 
+  (distinct_tar_reg (Arith (Binop bop r1 r2 ri))
+    ⇔ (r1 ≠ r2 ∧ case ri of (Reg r3) => r1 ≠ r3 | _ => T)) ∧
   (distinct_tar_reg  (Arith (Shift l r1 r2 n))
-    ⇔ r1 ≠ r2) ∧ 
+    ⇔ r1 ≠ r2) ∧
   (distinct_tar_reg _ ⇔ T)`
 
 (*Instructions are 2 register code for arith ok*)
 val two_reg_inst_def = Define`
-  (two_reg_inst (Arith (Binop bop r1 r2 ri)) 
-    ⇔ (r1 = r2)) ∧ 
+  (two_reg_inst (Arith (Binop bop r1 r2 ri))
+    ⇔ (r1 = r2)) ∧
   (two_reg_inst (Arith (Shift l r1 r2 n))
-    ⇔ (r1 = r2)) ∧ 
+    ⇔ (r1 = r2)) ∧
   (two_reg_inst _ ⇔ T)`
 
 (*TODO: move to HOL*)
@@ -265,19 +380,19 @@ val insert_shadow = prove(``
   rw[]>>
   simp[Once insert_def]>>
   simp[Once insert_def,SimpRHS]>>
-  `(a-1) DIV 2 < a` by 
+  `(a-1) DIV 2 < a` by
     (`0 < (2:num)` by fs[] >>
     imp_res_tac DIV_LT_X>>
     first_x_assum match_mp_tac>>
     DECIDE_TAC)>>
   metis_tac[])
- 
+
 (*Semantics preservation*)
 val three_to_two_reg_correct = prove(``
   ∀prog s res s'.
-  every_inst distinct_tar_reg prog ∧ 
+  every_inst distinct_tar_reg prog ∧
   evaluate (prog,s) = (res,s') ∧ res ≠ SOME Error
-  ⇒ 
+  ⇒
   evaluate(three_to_two_reg prog,s) = (res,s')``,
   ho_match_mp_tac three_to_two_reg_ind>>
   rw[]>>fs[three_to_two_reg_def,evaluate_def,state_component_equality]>>
@@ -317,8 +432,8 @@ val three_to_two_reg_syn = prove(``
 
 (*word_alloc preserves all syntactic program convs*)
 val word_alloc_two_reg_inst_lem = prove(``
-  ∀f prog. 
-  every_inst two_reg_inst prog ⇒ 
+  ∀f prog.
+  every_inst two_reg_inst prog ⇒
   every_inst two_reg_inst (apply_colour f prog)``,
   ho_match_mp_tac apply_colour_ind>>fs[every_inst_def]>>rw[]
   >-
@@ -329,13 +444,13 @@ val word_alloc_two_reg_inst_lem = prove(``
 
 val word_alloc_two_reg_inst = prove(``
   ∀k prog.
-  every_inst two_reg_inst prog ⇒ 
+  every_inst two_reg_inst prog ⇒
   every_inst two_reg_inst (word_alloc k prog)``,
   fs[word_alloc_two_reg_inst_lem,word_alloc_def,LET_THM])
 
 val word_alloc_flat_exp_conventions_lem = prove(``
-  ∀f prog. 
-  flat_exp_conventions prog ⇒ 
+  ∀f prog.
+  flat_exp_conventions prog ⇒
   flat_exp_conventions (apply_colour f prog)``,
   ho_match_mp_tac apply_colour_ind>>fs[flat_exp_conventions_def]>>rw[]
   >-
@@ -345,14 +460,14 @@ val word_alloc_flat_exp_conventions_lem = prove(``
 
 val word_alloc_flat_exp_conventions = prove(``
   ∀k prog.
-  flat_exp_conventions prog ⇒ 
+  flat_exp_conventions prog ⇒
   flat_exp_conventions (word_alloc k prog)``,
   fs[word_alloc_flat_exp_conventions_lem,word_alloc_def,LET_THM])
 
 val fake_moves_flat_exp_conventions = prove(``
   ∀ls ssal ssar na l r a b c.
-  fake_moves ls ssal ssar na = (l,r,a,b,c) ⇒ 
-  flat_exp_conventions l ∧ 
+  fake_moves ls ssal ssar na = (l,r,a,b,c) ⇒
+  flat_exp_conventions l ∧
   flat_exp_conventions r``,
   Induct>>fs[fake_moves_def]>>rw[]>>fs[flat_exp_conventions_def]>>
   pop_assum mp_tac>> LET_ELIM_TAC>> EVERY_CASE_TAC>> fs[LET_THM]>>unabbrev_all_tac>>
