compiler/backend/word_to_targetScript.sml
@@ -19,9 +19,9 @@ Order of compilation (and their status):
 (*TODO: Maybe chain the max vars in a neater way instead of recomputing*)
 (*TODO: probably need to change reg_count to handle the restricted regs*)
 val compile_single_def = Define`
-  compile_single two_reg_arith reg_count (name_num:num,arg_count,prog) =
+  compile_single two_reg_arith reg_count c (name_num:num,arg_count,prog) =
   let maxv = max_var prog + 1 in
-  let inst_prog = inst_select maxv prog in
+  let inst_prog = inst_select c maxv prog in
   let ssa_prog = full_ssa_cc_trans arg_count inst_prog in
   let prog = if two_reg_arith then three_to_two_reg ssa_prog
                               else ssa_prog in
@@ -32,12 +32,12 @@ val compile_single_def = Define`
 
 val get_conf_props_def = Define `
   get_conf_props ((f,sp,bp,(c,enc,l)):'a stack_conf) =
-    (c.two_reg_arith, c.reg_count - 4)`;
+    (c.two_reg_arith, c.reg_count - 4,c)`;
 
 val compile_def = Define `
   compile start (conf:'a stack_conf) prog =
-    let (two_reg_arith,reg_count) = get_conf_props conf in
-    let prog = MAP (compile_single two_reg_arith reg_count) prog in
+    let (two_reg_arith,reg_count,c) = get_conf_props conf in
+    let prog = MAP (compile_single two_reg_arith reg_count c) prog in
       stack_to_target$compile start conf prog`
 
 val _ = export_theory ();
